Verity/Macro/Syntax.lean
@@ -16,6 +16,7 @@ declare_syntax_cat verityLocalObligations
 declare_syntax_cat verityConstructor
 declare_syntax_cat verityMutability
 declare_syntax_cat verityInitGuard
+declare_syntax_cat verityModifies
 declare_syntax_cat veritySpecialEntrypoint
 declare_syntax_cat verityFunction
 
@@ -33,6 +34,7 @@ syntax ident " := " ident ppSpace str : verityLocalObligation
 syntax "local_obligations " "[" sepBy(verityLocalObligation, ",") "]" : verityLocalObligations
 syntax "payable" : verityMutability
 syntax "view" : verityMutability
+syntax "modifies(" sepBy(ident, ",") ")" : verityModifies
 syntax "initializer(" ident ")" : verityInitGuard
 syntax "reinitializer(" ident ", " num ")" : verityInitGuard
 syntax "ecmCall " term:max ppSpace term:max : term
@@ -45,7 +47,7 @@ syntax "constructor " "(" sepBy(verityParam, ",") ")" (ppSpace verityLocalObliga
 syntax "constructor " "(" sepBy(verityParam, ",") ")" " payable" (ppSpace verityLocalObligations)? " := " term : verityConstructor
 syntax "receive" (ppSpace verityLocalObligations)? " := " term : veritySpecialEntrypoint
 syntax "fallback" (ppSpace verityLocalObligations)? " := " term : veritySpecialEntrypoint
-syntax "function " verityMutability* ident " (" sepBy(verityParam, ",") ")" (ppSpace verityInitGuard)? (ppSpace verityLocalObligations)? " : " term " := " term : verityFunction
+syntax "function " verityMutability* ident " (" sepBy(verityParam, ",") ")" (ppSpace verityInitGuard)? (ppSpace verityModifies)? (ppSpace verityLocalObligations)? " : " term " := " term : verityFunction
 
 syntax (name := verityContractCmd)
   "verity_contract " ident " where "
